rewritten with new inference rules and CompCert PTree

sva_ast.v
@@ -2,10 +2,11 @@
 
 (** Contains definitions for the "SVA" language. *)
 
-Require Export SfLib.
+Add LoadPath "./CompCert-Toolkit".
+Require Import Coqlib.
 
-Definition var := id.
-Definition nodevar := id.
+Definition var := positive.
+Definition nodevar := positive.
 
 Inductive value : Type :=
   | Uninit : value
@@ -17,8 +18,7 @@ Inductive tipe : Type :=
   | Char_t : tipe
   | Unknown_t : tipe
   | Pts_t : tipe -> nodevar -> tipe
-  | Handle_t : nodevar -> tipe -> tipe
-  | Assoc_t : nodevar -> tipe -> tipe.
+  | Handle_t : nodevar -> tipe -> tipe.
 
 Inductive binop : Type :=
   | Plus : binop
