sva_typing.v
@@ -1,7 +1,9 @@
+Add LoadPath "./CompCert-Toolkit".
 Require Export sva_ast.
+Require Export Maps.
 
-Definition varmap := partial_map tipe.
-Definition regionmap := partial_map tipe.
+Definition varmap := PTree.t tipe.
+Definition regionmap := PTree.t tipe.
 Definition context := prod varmap regionmap.
 
 (** TODO: lots of shit ...
@@ -12,7 +14,7 @@ Definition context := prod varmap regionmap.
 Inductive has_type_exp : context -> exp -> tipe -> Prop :=
   | SS0 : forall Gamma Delta x tau, 
       wf_context (Gamma,Delta) tau ->
-      Gamma x = Some tau ->
+      PTree.get x Gamma = Some tau ->
       has_type_exp (Gamma,Delta) (Var x) tau
   | SS1 : forall C n,
       has_type_exp C (Val (Int n)) Int_t
@@ -24,45 +26,45 @@ Inductive has_type_exp : context -> exp -> tipe -> Prop :=
       wf_context C tau ->
       tau = Int_t \/ tau = Char_t \/ tau = Unknown_t \/ tau = (Pts_t rho' tau') ->
       has_type_exp C (Val Uninit) tau
-  | SS4 : forall C e tau tau' rho rho',
-      has_type_exp C e (Pts_t tau rho) ->
+  | SS4 : forall Gamma Delta e tau tau' rho rho',
+      has_type_exp (Gamma,Delta) e (Pts_t tau rho) ->
       tau = Int_t \/ tau = (Pts_t tau' rho') \/ tau = (Handle_t rho' tau') ->
-      wf_context C (Assoc_t rho tau) ->
-      has_type_exp C (Load e) tau
-  | SS4char : forall C e rho,
-      has_type_exp C e (Pts_t Char_t rho) ->
-      wf_context C (Assoc_t rho Char_t) ->
-      has_type_exp C (Loadc e) Char_t
-  | SS5 : forall C e2 x tau rho,
-      has_type_exp C e2 (Pts_t tau rho) ->
-      wf_context C (Assoc_t rho Unknown_t) ->
-      has_type_exp C x (Handle_t rho Unknown_t) ->
-      has_type_exp C (LoadFromU x e2) Int_t
-  | SS5char : forall C e2 x tau rho,
-      has_type_exp C e2 (Pts_t tau rho) ->
-      wf_context C (Assoc_t rho Unknown_t) ->
-      has_type_exp C x (Handle_t rho Unknown_t) ->
-      has_type_exp C (LoadcFromU x e2) Char_t
-  | SS6 : forall C e2 x tau rho,
-      wf_context C (Assoc_t rho tau) ->
-      has_type_exp C x (Handle_t rho tau) ->
-      has_type_exp C e2 Int_t ->
-      has_type_exp C (PoolAlloc x e2) (Pts_t tau rho)
-  | SS7 : forall C e x tau rho,
-      wf_context C (Assoc_t rho tau) ->
-      has_type_exp C x (Handle_t rho tau) ->
-      has_type_exp C e Int_t -> 
-      has_type_exp C (CastI2Ptr x e (Pts_t tau rho)) (Pts_t tau rho)
+      PTree.get rho Delta = Some tau ->
+      has_type_exp (Gamma,Delta) (Load e) tau
+  | SS4char : forall Gamma Delta e rho,
+      has_type_exp (Gamma,Delta) e (Pts_t Char_t rho) ->
+      PTree.get rho Delta = Some Char_t ->
+      has_type_exp (Gamma,Delta) (Loadc e) Char_t
+  | SS5 : forall Gamma Delta e2 x tau rho,
+      has_type_exp (Gamma,Delta) e2 (Pts_t tau rho) ->
+      PTree.get rho Delta = Some Unknown_t ->
+      has_type_exp (Gamma,Delta) x (Handle_t rho Unknown_t) ->
+      has_type_exp (Gamma,Delta) (LoadFromU x e2) Int_t
+  | SS5char : forall Gamma Delta e2 x tau rho,
+      has_type_exp (Gamma,Delta) e2 (Pts_t tau rho) ->
+      PTree.get rho Delta = Some Unknown_t ->
+      has_type_exp (Gamma,Delta) x (Handle_t rho Unknown_t) ->
+      has_type_exp (Gamma,Delta) (LoadcFromU x e2) Char_t
+  | SS6 : forall Gamma Delta e2 x tau rho,
+      PTree.get rho Delta = Some tau ->
+      has_type_exp (Gamma,Delta) x (Handle_t rho tau) ->
+      has_type_exp (Gamma,Delta) e2 Int_t ->
+      has_type_exp (Gamma,Delta) (PoolAlloc x e2) (Pts_t tau rho)
+  | SS7 : forall Gamma Delta e x tau rho,
+      PTree.get rho Delta = Some tau ->
+      has_type_exp (Gamma,Delta) x (Handle_t rho tau) ->
+      has_type_exp (Gamma,Delta) e Int_t -> 
+      has_type_exp (Gamma,Delta) (CastI2Ptr x e (Pts_t tau rho)) (Pts_t tau rho)
   | SS8 : forall C e tau tau' rho,
-      wf_context C tau' ->
+      wf_context C (Pts_t tau' rho) ->
       has_type_exp C e (Pts_t tau rho) ->
       has_type_exp C (Cast e (Pts_t tau' rho)) (Pts_t tau' rho)
-  | SS9 : forall C e2 e3 x tau rho,
-      wf_context C (Assoc_t rho tau) ->
-      has_type_exp C x (Handle_t rho tau) ->
-      has_type_exp C e2 (Pts_t tau rho) ->
-      has_type_exp C e3 Int_t ->
-      has_type_exp C (Addr x e2 e3) (Pts_t tau rho)
+  | SS9 : forall Gamma Delta  e2 e3 x tau rho,
+      PTree.get rho Delta = Some tau ->
+      has_type_exp (Gamma,Delta) x (Handle_t rho tau) ->
+      has_type_exp (Gamma,Delta) e2 (Pts_t tau rho) ->
+      has_type_exp (Gamma,Delta) e3 Int_t ->
+      has_type_exp (Gamma,Delta) (Addr x e2 e3) (Pts_t tau rho)
   | SS10 : forall C e tau tau' rho',
       has_type_exp C e tau ->
       tau = Int_t \/ tau = Char_t \/ tau = Unknown_t \/ tau = (Pts_t rho' tau') ->
@@ -80,38 +82,38 @@ with has_type_stmt : context -> stmt -> Prop :=
       has_type_exp C (Var x) tau ->
       has_type_exp C e tau ->
       has_type_stmt C (Assign x e) 
-  | SS14 : forall C e1 e2 rho rho' tau tau',
-      wf_context C (Assoc_t rho tau) ->
-      has_type_exp C e1 (Pts_t tau rho) ->
-      has_type_exp C e2 tau ->
+  | SS14 : forall Gamma Delta e1 e2 rho rho' tau tau',
+      PTree.get rho Delta = Some tau ->
+      has_type_exp (Gamma,Delta) e1 (Pts_t tau rho) ->
+      has_type_exp (Gamma,Delta) e2 tau ->
       tau = Int_t \/ tau = (Pts_t tau' rho') \/ tau = (Handle_t rho' tau') ->
-      has_type_stmt C (Store e2 e1)
-  | SS14char : forall C e1 e2 rho,
-      wf_context C (Assoc_t rho Char_t) ->
-      has_type_exp C e1 (Pts_t Char_t rho) ->
-      has_type_exp C e2 Char_t ->
-      has_type_stmt C (Storec e2 e1)
-  | SS15 : forall C e1 e2 x rho tau,
-      wf_context C (Assoc_t rho Unknown_t) ->
-      has_type_exp C e1 (Pts_t tau rho) ->
-      has_type_exp C e2 tau ->
-      has_type_exp C x (Handle_t rho Unknown_t) ->
-      has_type_stmt C (StoreToU x e2 e1)
-  | SS15char : forall C e1 e2 x rho tau,
-      wf_context C (Assoc_t rho Unknown_t) ->
-      has_type_exp C e1 (Pts_t tau rho) ->
-      has_type_exp C e2 Char_t ->
-      has_type_exp C x (Handle_t rho Unknown_t) ->
-      has_type_stmt C (StorecToU x e2 e1)
-  | SS16 : forall C e2 x rho tau,
-      wf_context C (Assoc_t rho tau) ->
-      has_type_exp C (Var x) (Handle_t rho tau) ->
-      has_type_exp C e2 (Pts_t tau rho) ->
-      has_type_stmt C (PoolFree (Var x) e2)
+      has_type_stmt (Gamma,Delta) (Store e2 e1)
+  | SS14char : forall Gamma Delta e1 e2 rho,
+      PTree.get rho Delta = Some Char_t ->
+      has_type_exp (Gamma,Delta) e1 (Pts_t Char_t rho) ->
+      has_type_exp (Gamma,Delta) e2 Char_t ->
+      has_type_stmt (Gamma,Delta) (Storec e2 e1)
+  | SS15 : forall Gamma Delta e1 e2 x rho tau,
+      PTree.get rho Delta = Some Unknown_t ->
+      has_type_exp (Gamma,Delta) e1 (Pts_t tau rho) ->
+      has_type_exp (Gamma,Delta) e2 tau ->
+      has_type_exp (Gamma,Delta) x (Handle_t rho Unknown_t) ->
+      has_type_stmt (Gamma,Delta) (StoreToU x e2 e1)
+  | SS15char : forall Gamma Delta e1 e2 x rho tau,
+      PTree.get rho Delta = Some Unknown_t ->
+      has_type_exp (Gamma,Delta) e1 (Pts_t tau rho) ->
+      has_type_exp (Gamma,Delta) e2 Char_t ->
+      has_type_exp (Gamma,Delta) x (Handle_t rho Unknown_t) ->
+      has_type_stmt (Gamma,Delta) (StorecToU x e2 e1)
+  | SS16 : forall Gamma Delta e2 x rho tau,
+      PTree.get rho Delta = Some tau ->
+      has_type_exp (Gamma,Delta) (Var x) (Handle_t rho tau) ->
+      has_type_exp (Gamma,Delta) e2 (Pts_t tau rho) ->
+      has_type_stmt (Gamma,Delta) (PoolFree (Var x) e2)
   | SS17 : forall Gamma Delta s x rho tau,
       wf_context (Gamma,Delta) tau ->
-      Gamma x = None /\ Delta rho = None ->
-      has_type_stmt ((extend Gamma x (Handle_t rho tau)),(extend Delta rho tau)) s ->
+      PTree.get x Gamma = None /\ PTree.get rho Delta = None ->
+      has_type_stmt ((PTree.set x (Handle_t rho tau) Gamma),(PTree.set rho tau Delta)) s ->
       has_type_stmt (Gamma,Delta) (PoolInit rho tau x s)
 
 (* C |- tau *)
@@ -120,18 +122,19 @@ with wf_context : context -> tipe -> Prop :=
       wf_context C Int_t
   | SS19 : forall C,
       wf_context C Unknown_t
-  | SS20 : forall Gamma Delta rho tau,
-      Delta rho = Some tau ->
-      wf_context (Gamma,Delta) (Assoc_t rho tau)
-  | SS21 : forall C rho tau,
-      wf_context C (Assoc_t rho tau) ->
-      wf_context C (Pts_t tau rho)
-  | SS22 : forall Gamma Delta tau rho,
-      Delta rho = Some Unknown_t ->
+  (* SS20 was removed *)
+  | SS21 : forall Gamma Delta rho tau,
+      PTree.get rho Delta = Some tau ->
+      wf_context (Gamma,Delta) tau ->
       wf_context (Gamma,Delta) (Pts_t tau rho)
-  | SS23 : forall C rho tau,
-      wf_context C (Assoc_t rho tau) ->
-      wf_context C (Handle_t rho tau)
+  | SS22 : forall Gamma Delta tau rho,
+      PTree.get rho Delta = Some Unknown_t ->
+      wf_context (Gamma,Delta) tau ->
+      wf_context (Gamma,Delta) (Pts_t tau rho)
+  | SS23 : forall Gamma Delta rho tau,
+      PTree.get rho Delta = Some tau ->
+      wf_context (Gamma,Delta) tau ->
+      wf_context (Gamma,Delta) (Handle_t rho tau)
   | SS24 : forall C,
       wf_context C Char_t.
 
