sva_soundness.v
@@ -1,0 +1,25 @@
+Require Export sva_typing.
+Require Export SfLib.
+
+Tactic Notation "exp_cases" tactic(first) ident(c) :=
+  first;
+  [ Case_aux c "SS0" | Case_aux c "SS1" | Case_aux c "SS2"
+  | Case_aux c "SS3" | Case_aux c "SS4" | Case_aux c "SS4char"
+  | Case_aux c "SS5" | Case_aux c "SS5char" | Case_aux c "SS6"
+  | Case_aux c "SS7" | Case_aux c "SS8" | Case_aux c "SS9"
+  | Case_aux c "SS10" ].
+
+Lemma wf_type : forall (c : context) (e : exp) (tau : tipe),
+  has_type_exp c e tau -> wf_context c tau.
+Proof.
+  intros c e tau H. 
+  exp_cases (induction H) Case;
+  try (constructor; apply H).
+  Case "SS0". apply H.
+  Case "SS3". apply H.
+  Case "SS4". inversion IHhas_type_exp. apply H7. apply H7.
+  Case "SS6". inversion IHhas_type_exp1. constructor. apply H5. apply H7.
+  Case "SS7". inversion IHhas_type_exp1. constructor. apply H5. apply H7.
+  Case "SS8". apply H.
+  Case "SS9". apply IHhas_type_exp2.
+Qed.
